Added Ictr, EWflag and ORset MRDT

icounter.fst
@@ -1,89 +1,230 @@
 module Icounter
 
 open FStar.List.Tot
-open History
 
-type o =
-  | Inc : nat -> o
+type op =
+     | Inc : nat -> op
+
+type o = (nat (*unique id*) * op)
 
 type s = nat
-
+     
 val app_op : s -> o -> s
-let app_op s (Inc n) = s + n
-
-instance icounter : datatype s o = {
-  History.apply_op = app_op
-}
-
-val le : nat -> nat -> bool
-let le a b = a <= b
-
-val lemma1 : tr:list o -> s1:s
-           -> Lemma (ensures (le s1 (fold_left apply_op s1 tr)))
-let rec lemma1 tr s1 =
-  match tr with
-  | [] -> ()
-  | op::ops ->
-     let s2 = app_op s1 op in
-     lemma1 ops s2
-
-val lemma2 : l1:nat -> l2:nat -> lab:nat  -> lbc:nat -> lac:nat  -> a:nat  -> b:nat -> c:nat 
-             -> Lemma (requires l1 = l2)
-                     (ensures (a + (b + c - lbc) - (lab + lac - l2)) = ((a + b - lab) + c - (lbc + lac - l1)))
-let lemma2 l1 l2 lab lbc lac a b c = ()
-
-val merge : a:history s o
-          -> b:history s o
-          -> l:history s o{wellformed l /\ is_lca l a b}
-          -> s
-let merge a b l = 
-  History.lemma1 l;
-  assert (wellformed a);
-
-  let tr = get_trace l a in
-  assert (fold_left apply_op (get_state l) tr = get_state a);
-
-  lemma1 tr (get_state l);
-  assert (get_state a >= get_state l);
-
-  get_state a + get_state b - get_state l
-
-val commutativity : a:history s o
-                  -> b:history s o
-                  -> l:history s o{wellformed l /\ is_lca l a b}
-                  -> Lemma (ensures (merge a b l = merge b a l))
-let commutativity a b l = ()
-
-val idempotence : a:history s o{wellformed a /\ is_lca a a a}
-                -> Lemma (ensures (merge a a a = get_state a))
-let idempotence a = ()
-
-val associativity : h:history s o{wellformed h}
-                -> a:history s o{wellformed a /\ hbeq h a}
-                -> b:history s o{wellformed b /\ hbeq h b}
-                -> c:history s o{wellformed c /\ hbeq h c}
-                -> lab:history s o{lcau h a b = lab}
-                -> lbc:history s o{lcau h b c = lbc}
-                -> lac:history s o{lcau h c a = lac}
-                -> mab:history s o{hbeq h mab /\ merge_node a b mab /\ get_state mab = merge a b lab}
-                -> mbc:history s o{hbeq h mbc /\ merge_node b c mbc /\ get_state mbc = merge b c lbc}
-                -> m1:history s o{hbeq h m1 /\ merge_node lab lac m1 /\ get_state m1 = merge lab lac (lcau h lab lac) /\ lcau h a mbc = m1}
-                -> m2:history s o{hbeq h m2 /\ merge_node lbc lac m2 /\ get_state m2 = merge lbc lac (lcau h lbc lac) /\ lcau h mab c = m2}
-                -> mabc1: history s o{hbeq h mabc1 /\ merge_node a mbc mabc1 /\ get_state mabc1 = merge a mbc m1}
-                -> mabc2: history s o{hbeq h mabc2 /\ merge_node mab c mabc2 /\ get_state mabc2 = merge mab c m2}
-                -> Lemma (get_state mabc1 = get_state mabc2)
-                
-let associativity h a b c lab lbc lac mab mbc m1 m2 mabc1 mabc2 = 
-  lcau_associative h a b c lab lbc lac;
-  let l2 = lcau h lab lac in
-  let l1 = lcau h lbc lac in
-  lemma2 (get_state l1) (get_state l2) (get_state lab) (get_state lbc) (get_state lac) (get_state a) (get_state b) 
-         (get_state c); ()
+let app_op c (_,Inc n) = c + n
   
+val member : id:nat 
+           -> l:list o
+           -> Tot (b:bool{(exists n. mem (id,n) l) <==> b=true})
+let rec member n l =
+  match l with
+  |[] -> false
+  |(id,_)::xs -> (n = id) || member n xs
 
-instance _ : mrdt s o icounter = {
-  History.merge = merge;
-  History.commutativity = commutativity;
-  History.idempotence = idempotence;
-  History.associativity = associativity
-}
+val unique : l:list o
+           -> Tot bool
+let rec unique l =
+  match l with
+  |[] -> true
+  |(id,_)::xs -> not (member id xs) && unique xs
+
+noeq type ae  =
+     |A : vis : (o -> o -> Tot bool)
+        -> l:(list o) {(forall e e' e''. (mem e l /\ mem e' l /\ mem e'' l /\ vis e e' /\ vis e' e'') ==> vis e e'') (*transitive*)/\ 
+                      (forall e e'. (mem e l /\ mem e' l /\ vis e e') ==> not (vis e' e)) (*asymmetric*) /\
+                      (forall e. mem e l ==> not (vis e e) (*irreflexive*) /\
+                      (unique l))}  
+        -> ae
+
+val sum : a:(list o) -> Tot nat (decreases a)
+let rec sum l =
+  match l with
+  |[] -> 0
+  |((_,Inc n)::xs) -> n + sum xs
+
+#set-options "--query_stats"              
+val sim : tr:ae
+        -> s1:s 
+        -> Tot bool        
+let sim tr s1 = (s1 = sum tr.l)
+
+val rem1 : l:ae 
+         -> op:o
+         -> Pure (list o)
+           (requires true)
+           (ensures (fun r -> (forall n. ((snd op = (Inc n) /\ mem op l.l /\ l.l <> []) ==> (sum r = sum l.l - n))) /\ 
+                           (forall ele. mem ele r ==> mem ele l.l) /\ (unique r))) (decreases %[l.l])
+let rec rem1 l op =
+    match l with 
+    |(A _ []) -> []
+    |(A _ (x::xs)) -> if (x = op) then xs else (x::(rem1 (A l.vis xs) op))
+          
+val rem : l:ae 
+        -> op:o 
+        -> Pure ae
+          (requires true)
+          (ensures (fun r -> (forall n. ((snd op = (Inc n) /\ mem op l.l /\ l.l <> []) ==> (sum r.l = sum l.l - n))) /\ 
+                          (forall e. mem e r.l ==> mem e l.l) /\
+                          (forall e e1. mem e r.l /\ mem e1 r.l /\ r.vis e e1 ==> mem e l.l /\ mem e1 l.l /\ l.vis e e1)))
+let rem l op =
+  let res = (rem1 l op) in
+  (A (fun o o1 -> mem o l.l && mem o1 l.l && l.vis o o1) res)
+
+val diff1 : a:ae
+          -> l:ae
+          -> Pure (list o)
+            (requires (forall e. mem e l.l ==> mem e a.l) /\ 
+                      (forall e e1. mem e l.l /\ mem e1 l.l /\ l.vis e e1 ==> mem e a.l /\ mem e1 a.l /\ a.vis e e1) /\
+                      (forall e e1. (mem e l.l /\ mem e1 a.l ==> mem e a.l /\ a.vis e e1)))
+            (ensures (fun d -> (forall e. mem e d <==> mem e a.l /\ not (mem e l.l)) /\
+                            (sum d = sum a.l - sum l.l) /\
+                            (forall e. mem e d ==> not (member (fst e) l.l)))) (decreases %[l.l;a.l])
+let rec diff1 a l = 
+    match a,l with
+    |_,(A _ []) -> a.l
+    |_,(A _ (x::xs)) -> if (mem x a.l) then (diff1 (rem a x) (A l.vis xs)) else (diff1 a (A l.vis xs))
+
+val diff : a:ae
+         -> l:ae
+         -> Pure ae
+          (requires (forall e. mem e l.l ==> mem e a.l) /\ 
+                    (forall e e1. mem e l.l /\ mem e1 l.l /\ l.vis e e1 ==> mem e a.l /\ mem e1 a.l /\ a.vis e e1) /\
+                    (forall e e1. (mem e l.l /\ mem e1 a.l ==> mem e a.l /\ a.vis e e1)))
+          (ensures (fun d -> (forall e. mem e d.l <==> mem e a.l /\ not(mem e l.l)) /\
+                          (sum d.l = sum a.l - sum l.l) /\
+                          (forall e. mem e d.l ==> not (member (fst e) l.l)) /\
+                          (forall e e1. mem e d.l /\ mem e1 d.l /\ d.vis e e1 ==> mem e a.l /\ mem e1 a.l /\ a.vis e e1))) (decreases l)
+let diff a l =
+  (A (fun o o1 -> mem o a.l && mem o1 a.l && a.vis o o1) (diff1 a l))
+
+val union1 : a:ae 
+           -> b:ae
+           -> Pure (list o)
+             (requires (forall e. (mem e a.l ==> not (member (fst e) b.l))) /\
+                             (forall e. (mem e b.l ==> not (member (fst e) a.l))))
+             (ensures (fun u -> (sum u = sum a.l + sum b.l) /\ 
+                             (forall e. mem e u <==> mem e a.l \/ mem e b.l) /\
+                             (unique u)))     (decreases %[a.l;b.l])        
+let rec union1 a b =
+  match a,b with
+  |(A _ []),(A _ []) -> []
+  |(A _ (x::xs)),_ -> x::(union1 (A (fun o o1 -> mem o a.l && mem o1 a.l && a.vis o o1) xs) b)
+  |(A _ []), (A _ (x::xs)) -> x::(union1 a (A (fun o o1 -> mem o b.l && mem o1 b.l && b.vis o o1) xs))
+
+val union : a:ae 
+          -> b:ae
+          -> Pure ae
+            (requires (forall e. (mem e a.l ==> not (member (fst e) b.l))) /\
+                            (forall e. (mem e b.l ==> not (member (fst e) a.l))))
+            (ensures (fun u -> (sum u.l = sum a.l + sum b.l) /\ 
+                            (forall e. mem e u.l <==> mem e a.l \/ mem e b.l) /\
+                            (forall e e1. (mem e u.l /\ mem e1 u.l /\ u.vis e e1) <==> 
+                                     ((mem e a.l /\ mem e1 a.l /\ a.vis e e1) \/ (mem e b.l /\ mem e1 b.l /\ b.vis e e1)))))
+let union a b = 
+  (A (fun o o1 -> (mem o a.l && mem o1 a.l && a.vis o o1) || (mem o b.l && mem o1 b.l && b.vis o o1)) (union1 a b))
+  
+val absmerge : l:ae
+             -> a:ae
+             -> b:ae
+             -> Pure ae 
+               (requires (forall e. mem e l.l <==> mem e a.l /\ mem e b.l) /\ 
+                         (forall e1 e2. mem e1 l.l /\ mem e2 l.l /\ l.vis e1 e2 <==> 
+                                   mem e1 a.l /\ mem e2 a.l /\ a.vis e1 e2 /\ mem e1 b.l /\ mem e2 b.l /\ b.vis e1 e2) /\
+                         (forall e e1. mem e l.l /\ mem e1 a.l ==> a.vis e e1) /\
+                         (forall e e1. mem e l.l /\ mem e1 b.l ==> b.vis e e1) /\
+                         (forall e. mem e (diff a l).l ==> not (member (fst e) b.l)) /\
+                         (forall e1. mem e1 (diff b l).l ==> not (member (fst e1) a.l)))  
+                (ensures (fun u -> (forall e. mem e u.l <==> mem e l.l \/ mem e a.l \/ mem e b.l) /\ 
+                               (forall e1 e2. (mem e1 u.l /\ mem e2 u.l /\ u.vis e1 e2) <==> 
+                                         (mem e1 l.l /\ mem e2 l.l /\ l.vis e1 e2) \/
+                                         (mem e1 a.l /\ mem e2 a.l /\ a.vis e1 e2) \/ 
+                                         (mem e1 b.l /\ mem e2 b.l /\ b.vis e1 e2))))
+                                       
+let absmerge l a b = 
+    let la = diff a l in
+    let lb = diff b l in
+    let u1 = union la lb in
+    let res = union l u1 in
+    (A (fun o o1 -> (mem o l.l && mem o1 l.l && l.vis o o1) || 
+                 (mem o a.l && mem o1 a.l && a.vis o o1) || 
+                 (mem o b.l && mem o1 b.l && b.vis o o1)) res.l)
+
+val lemma : ltr:ae 
+          -> l:s 
+          -> atr:ae 
+          -> a:s 
+          -> Lemma (ensures (sim ltr l /\ sim atr a /\
+                           (forall e. mem e ltr.l ==> mem e atr.l) /\
+                           (forall e e1. mem e ltr.l /\ mem e1 atr.l  ==> mem e atr.l /\ atr.vis e e1)) ==> a >= l)
+                           (decreases %[ltr.l;atr.l])
+let rec lemma ltr l atr a = 
+  match ltr,atr with
+  |(A _ []), (A _ []) -> ()
+  |(A _ (x::xs)), _ -> lemma (A ltr.vis xs) l atr a
+  |(A _ []), (A _ (x::xs)) -> lemma ltr l (A atr.vis xs) a
+
+val merge : ltr:ae
+          -> l:s
+          -> atr:ae
+          -> a:s 
+          -> btr:ae
+          -> b:s 
+          -> Pure s (requires (sim ltr l /\ sim atr a /\ sim btr b) /\ 
+                             (forall e. mem e ltr.l <==> mem e atr.l /\ mem e btr.l) /\
+                             (forall e e1. mem e ltr.l /\ mem e1 atr.l ==> mem e atr.l /\ atr.vis e e1) /\
+                             (forall e e1. mem e ltr.l /\ mem e1 btr.l ==>  mem e btr.l /\ btr.vis e e1) /\
+                             (forall e1 e2. (mem e1 ltr.l /\ mem e2 ltr.l /\ ltr.vis e1 e2) <==> 
+                                       (mem e1 atr.l /\ mem e2 atr.l /\ atr.vis e1 e2 /\ 
+                                        mem e1 btr.l /\ mem e2 btr.l /\ btr.vis e1 e2)) /\
+                             (forall e e1. mem e (diff atr ltr).l /\ mem e1 (diff btr ltr).l ==> 
+                                      not (member (fst e) btr.l) /\ not (member (fst e1) atr.l)))                
+                   (ensures (fun res -> true))                  
+let merge ltr l atr a btr b = 
+    lemma ltr l atr a;
+    lemma ltr l btr b;
+    a + b - l
+
+val append : tr:ae
+           -> op:o
+           -> Pure ae
+             (requires (not (member (fst op) tr.l)))
+             (ensures (fun res -> true)) (decreases tr.l)               
+let append tr op =
+    match tr with
+    |(A _ []) -> (A (fun o o1 -> mem o tr.l && mem o1 tr.l && tr.vis o o1) (op::[]))
+    |(A _ (x::xs)) -> (A (fun o o1 -> mem o tr.l && mem o1 tr.l && tr.vis o o1) (op::(x::xs)))
+
+val prop_merge : ltr: ae
+               -> l:s 
+               -> atr:ae
+               -> a:s 
+               -> btr:ae
+               -> b:s 
+               -> Lemma (requires (sim ltr l /\ sim atr a /\ sim btr b) /\ 
+                                 (forall e. mem e ltr.l <==> mem e atr.l /\ mem e btr.l) /\
+                                 (forall e e1. mem e ltr.l /\ mem e1 atr.l ==> mem e atr.l /\ atr.vis e e1) /\
+                                 (forall e e1. mem e ltr.l /\ mem e1 btr.l ==> mem e btr.l /\ btr.vis e e1) /\
+                                 (forall e1 e2. (mem e1 ltr.l /\ mem e2 ltr.l /\ ltr.vis e1 e2) <==> 
+                                           (mem e1 atr.l /\ mem e2 atr.l /\ atr.vis e1 e2 /\ 
+                                           mem e1 btr.l /\ mem e2 btr.l /\ btr.vis e1 e2)) /\
+                                 (forall e e1. mem e (diff atr ltr).l /\ mem e1 (diff btr ltr).l ==> 
+                                          not (member (fst e) btr.l) /\ not (member (fst e1) atr.l)))                        
+                       (ensures (sim (absmerge ltr atr btr) (merge ltr l atr a btr b))) 
+
+#set-options "--z3rlimit 30"    
+let prop_merge ltr l atr a btr b = ()
+
+val prop_oper : tr:ae
+              -> st:s
+              -> op:o 
+              -> Lemma (requires (sim tr st) /\ 
+                                (not (member (fst op) tr.l)) /\ 
+                                (forall e. mem e tr.l ==> (append tr op).vis e op))
+                      (ensures (sim (append tr op) (app_op st op))) (decreases %[tr.l])
+let prop_oper tr st op = ()
+          
+val convergence : tr:ae
+                -> a:s 
+                -> b:s 
+                -> Lemma (ensures (sim tr a /\ sim tr b) ==> a = b)                      
+let convergence tr a b = ()
+
